# T1 - (Henrique Martins)

**A)**

$$
  X = \begin{bmatrix}
       2 & 2\\
       0 & 3
     \end{bmatrix}
$$

$$
  A = \begin{bmatrix}
       2 & 2\\
       1 & 2
     \end{bmatrix}
  , B = \begin{bmatrix}
      2 & -1\\
      -1 & 2
    \end{bmatrix}
$$

<br>

$$
X_{11} = (2 * 2 + 2 * -1) = 2
$$

$$
X_{12} = (2 * -1 + 2 * 2) = 2
$$

$$
X_{21} = (1 * 2 + 2 * -1) = 2
$$

$$
X_{22} = (1 * -1 + 2 * 2) = 2
$$

---

**B)**

$$
x = 2 - \frac{2 - 5 * \frac{5}{7}}{3} - (-\frac{5}{7}); y = \frac{2 - 5 * \frac{5}{7}}{3} - (-\frac{5}{7}); z = \frac{5}{7}
$$

<br>

$$
\begin{cases}
    x + y + z = 2 \\
    2x + y + 3z = 6 \\
    3x - y + 4z = 5
  \end{cases}
$$

<br>

$$
y = 6 - 2(2 - y - z) - 3z
$$

$$
y = 6 - 4 - 2y - 2z - 3z
$$

$$
y = 2 - 2y - 5z
$$

$$
y + 2y = 2 - 5z
$$

$$
3y = 2 - 5z
$$

$$
y = \frac{2 - 5z}{3}
$$

<br>

$$
4z = 5 - 3x + y
$$

$$
4z = 5 - 3(2 - y - z) + y
$$

$$
4z = 5 - 3(2 - \frac{2 - 5z}{3} - z) + \frac{2 - 5z}{3}
$$

<br>

$$
-3(2 - \frac{2 - 5z}{3} - z) = -3 * 2 -((\frac{2 - 5z}{3}) * \frac{-3}{1}) + 3z
$$

$$
-3 * 2 - ((\frac{2 - 5z}{3}) * \frac{-3}{1}) + 3z =-6 -(\frac{6 + 15z}{3}) + 3zz
$$

<br>

$$
4z = 5 - 6 - \frac{-6 + 15z}{3} + 3z + \frac{2 - 5z}{3}
$$

$$
4z - 3z = -1 - (\frac{-6 + 15z}{3}) + \frac{2 - 5z}{3}
$$

$$
4z - 3z = -1 - \frac{-6}{3} + \frac{-15z}{3} + \frac{2}{3} - \frac{5z}{3}
$$

$$
4z - 3z - \frac{15z}{3} + \frac{5z}{3} = -1 - \frac{-6}{3} + \frac{2}{3}
$$

$$
3 (4z - 3z - \frac{15z}{3} + \frac{5z}{3} = -1 - \frac{-6}{3} + \frac{2}{3})
$$

$$
3z - 15z + 5z = -3 - (-6) + 2
$$

$$
3z - 10z = -3 - (-6) + 2
$$

$$
-7z = -3 - (-6) + 2
$$

$$
-7z = -5
$$

$$
-z = \frac{5}{7}
$$

$$
z = -\frac{5}{7}
$$

$$
y = \frac{2 - 5z}{3}
$$

$$
y = \frac{2 - 5 * - \frac{5}{7}}{3}
$$

$$
y = 2 - \frac{2 - 5 * - \frac{5}{7}}{3} - (- \frac{5}{7})
$$
